Progress from Dec

examples/computability/kolmog/kraft_ineqScript.sml
@@ -31,23 +31,23 @@ val Fpow_def = Define`Fpow n = GENLIST (K F) n`
 val _ = set_mapped_fixity{fixity = Infix(NONASSOC,450),term_name = "prefix",tok="≺"}
 
 val prefix_refl = Q.store_thm("prefix_refl[simp]",
-`¬(l ≺ l)`,
+`~(l ≺ l)`,
 simp[prefix_def])
 
-val prefix_free_def = Define`prefix_free (s:α list set) = ∀a b. a ∈ s ∧ b∈s ==> ¬(a≺ b) `
+val prefix_free_def = Define`prefix_free (s:'a list set) = !a b. a IN s /\ b IN s ==> ~(a≺ b) `
 
 val prefix_free_empty = Q.store_thm("prefix_free_empty[simp]",
-`prefix_free ∅`,
+`prefix_free EMPTY `,
 rw[prefix_free_def])
 
 val prefix_free_sing = Q.store_thm("prefix_free_sing[simp]",
 `prefix_free {l}`,
 rw[prefix_free_def])
 
-val len_fun_def = Define`len_fun (A:bool list set) n = let strs = {s | (LENGTH s = n) ∧ s ∈ A} in EXTREAL_SUM_IMAGE (λs. Normal (2 rpow (- &(LENGTH s)))) strs`
+val len_fun_def = Define`len_fun (A:bool list set) n = let strs = {s | (LENGTH s = n) /\ s IN A} in EXTREAL_SUM_IMAGE (\s. Normal (2 rpow (- &(LENGTH s)))) strs`
 
 val extreal_sum_image_finite_corr = Q.store_thm("extreal_sum_image_finite_corr",
-`∀P. FINITE P ⇒ ∀f x. (∀y. (y ∈ P) ==> (f y = x)) ⇒ (SIGMA f P = &CARD P * x)`,
+`!P. FINITE P ==> !f x. (!y. (y IN P) ==> (f y = x)) ==> (SIGMA f P = &CARD P * x)`,
    REPEAT STRIP_TAC
    >> (MP_TAC o Q.SPECL [`P`]) extrealTheory.EXTREAL_SUM_IMAGE_FINITE_SAME
    >> RW_TAC std_ss []
@@ -69,7 +69,7 @@ val finite_bool_list_n = Q.store_thm("finite_bool_list_n[simp]",
 irule (INST_TYPE[beta|->``:num``] FINITE_INJ) >> qexists_tac`bool_list_to_num` >>
           qexists_tac`count (2**(n+1)-1)` >> simp[INJ_DEF] >> qid_spec_tac`n` >> Induct_on`x`>>
           simp[bool_list_to_num_def] >> pop_assum(qspec_then`LENGTH x` MP_TAC) >>rw[] >> 
-          simp[GSYM ADD1,Once EXP] >> irule (DECIDE``n<=2n ∧ b<x-1 ==> 2*b+n<2*x-1``) >> rw[ADD1])
+          simp[GSYM ADD1,Once EXP] >> irule (DECIDE``n<=2n /\ b<x-1 ==> 2*b+n<2*x-1``) >> rw[ADD1])
 
 val bool_list_card = Q.store_thm("bool_list_card[simp]",
 `CARD {s | LENGTH (s:bool list) = n} = 2**n`,
@@ -80,7 +80,7 @@ qmatch_abbrev_tac`(x:num)-y=x` >> `y=0`suffices_by simp[] >> simp[Abbr`y`,EXTENS
 metis_tac[]  )
 
 val len_fun_eq1 = Q.store_thm("len_fun_eq1",
-`SIGMA (λs. Normal (2 rpow -&LENGTH s)) {s | (LENGTH (s:bool list) = n)} = 1`,
+`SIGMA (\s. Normal (2 rpow -&LENGTH s)) {s | (LENGTH (s:bool list) = n)} = 1`,
 irule EQ_TRANS >>qexists_tac`&CARD {s | LENGTH (s:bool list) = n} * Normal(2 rpow (-&n))` >> conj_tac
   >- (irule extreal_sum_image_finite_corr >> rw[])
   >- (simp[extreal_of_num_def,extreal_mul_def,GSYM realTheory.REAL_OF_NUM_POW,GEN_RPOW,
@@ -88,8 +88,8 @@ irule EQ_TRANS >>qexists_tac`&CARD {s | LENGTH (s:bool list) = n} * Normal(2 rpo
 
 val len_fun_le1 = Q.store_thm("len_fun_le1",
 `len_fun A n <= 1`,
-rw[len_fun_def] >> `{s | LENGTH s = n ∧ s ∈ A}⊆{s|LENGTH s = n}` by simp[SUBSET_DEF] >> 
-`FINITE {s | LENGTH s = n ∧ s ∈ A}` by metis_tac[SUBSET_FINITE_I,finite_bool_list_n] >> 
+rw[len_fun_def] >> `{s | LENGTH s = n /\ s IN A} SUBSET {s|LENGTH s = n}` by simp[SUBSET_DEF] >> 
+`FINITE {s | LENGTH s = n /\ s IN A}` by metis_tac[SUBSET_FINITE_I,finite_bool_list_n] >> 
 ASSUME_TAC len_fun_eq1 >> pop_assum(SUBST1_TAC o SYM)>> irule EXTREAL_SUM_IMAGE_MONO_SET >> 
 simp[finite_bool_list_n] >> rw[extreal_of_num_def,extreal_le_def] >> 
 `0r < 2 `suffices_by(strip_tac >> drule RPOW_POS_LT >> simp[realTheory.REAL_LE_LT]) >>
@@ -105,13 +105,13 @@ val rev_tpow = Q.store_thm("rev_tpow[simp]",
 simp[Tpow_def,listTheory.REVERSE_GENLIST,combinTheory.K_DEF])
 
 
-val tbl2n_def = Define`tbl2n [] = 0n ∧ tbl2n (T::t) = 2*tbl2n t + 1 ∧ tbl2n (F::t) = 2*tbl2n t`
+val tbl2n_def = Define`tbl2n [] = 0n /\ tbl2n (T::t) = 2*tbl2n t + 1 /\ tbl2n (F::t) = 2*tbl2n t`
 
 val _ = export_rewrites["tbl2n_def"]
 
-val _ = overload_on("TBL2N",``λl. tbl2n (REVERSE l)``)
+val _ = overload_on("TBL2N",``\l. tbl2n (REVERSE l)``)
 
-val inv_tbl2n_def = tDefine"inv_tbl2n"`inv_tbl2n 0n = [] ∧ 
+val inv_tbl2n_def = tDefine"inv_tbl2n"`inv_tbl2n 0n = [] /\ 
                            inv_tbl2n a = if EVEN a 
                                          then [F]++(inv_tbl2n (a DIV 2))
                                          else [T]++(inv_tbl2n ((a-1) DIV 2 ))`
@@ -134,7 +134,7 @@ simp[tbl2n_def]
 val interval_bl_def = Define`interval_bl l = (&(TBL2N l) *(2 rpow -&LENGTH l),(2 rpow -&LENGTH l))`
 
 val disjoint_interval_def = Define`disjoint_interval ((m:real),i) (n,j) <=> 
-                                   DISJOINT {r|m<=r ∧ r<m+i} {r|n<=r ∧ r<n+j}`
+                                   DISJOINT {r|m<=r /\ r<m+i} {r|n<=r /\ r<n+j}`
 
 val tbl2n_exp2 = Q.store_thm("tbl2n_exp2",
 `tbl2n i * 2 ** n = tbl2n ((Fpow n)++i)`,
@@ -169,7 +169,7 @@ val tbl2n_append_1 = Q.store_thm("tbl2n_append_1",
 Induct_on`x` >> simp[] >- (Cases_on`e` >> simp[]) >> Cases_on`h` >> simp[] >> rw[] >> simp[EXP] );
 
 val tbl2n_append_full = Q.store_thm("tbl2n_append_full",
-`∀y. tbl2n (x++y) = tbl2n x + 2**(LENGTH x) * tbl2n y`,
+`!y. tbl2n (x++y) = tbl2n x + 2**(LENGTH x) * tbl2n y`,
 Induct_on`x` >> simp[] >> Cases_on`h` >> simp[EXP])
 
 val tbl2n_ub = Q.store_thm("tbl2n_ub[simp]",
@@ -182,17 +182,17 @@ metis_tac[tbl2n_ub,LENGTH_REVERSE]);
 
 
 val TBL2N_inj_len = Q.store_thm("TBL2N_inj_len",
-`∀x y.(LENGTH x = LENGTH y) ==> (TBL2N x = TBL2N y <=> x=y)`,
+`!x y.(LENGTH x = LENGTH y) ==> (TBL2N x = TBL2N y <=> x=y)`,
 Induct_on`x` >> simp[] >> Cases_on`y` >> simp[] >> rw[tbl2n_append_1] >> 
 `TBL2N t < 2** LENGTH t` by  (metis_tac[tbl2n_ub,LENGTH_REVERSE]) >>  
 `TBL2N x < 2** LENGTH t` by  (metis_tac[tbl2n_ub,LENGTH_REVERSE]) >>simp[]);
 
 val TBL2N_lem1 = Q.store_thm("TBL2N_lem1",
-`∀δ. δ<2**Δ ==> ∃l. TBL2N l = δ ∧ LENGTH l = Δ ∧ TBL2N (i++Fpow Δ) +δ = TBL2N (i++l)`,
-Induct_on`Δ` >- simp[Fpow_def] >> rw[EXP] >> Cases_on`δ<2**Δ` >> fs[]
+`!d. d<2**D ==> ?l. TBL2N l = d /\ LENGTH l = D /\ TBL2N (i++Fpow D) +d = TBL2N (i++l)`,
+Induct_on`D` >- simp[Fpow_def] >> rw[EXP] >> Cases_on`d<2**D` >> fs[]
   >- (res_tac >> qexists_tac`F::l` >> simp[] >> fs[REVERSE_APPEND] >> simp[tbl2n_append_full])
-  >- (qabbrev_tac`δ0=δ-2**Δ` >> `δ0 < 2**Δ` by simp[Abbr`δ0`] >> res_tac >> qexists_tac`T::l` >>
-      simp[] >>fs[REVERSE_APPEND] >> simp[tbl2n_append_full] >> simp[Abbr`δ0`] ) )
+  >- (qabbrev_tac`d0=d-2**D` >> `d0 < 2**D` by simp[Abbr`d0`] >> res_tac >> qexists_tac`T::l` >>
+      simp[] >>fs[REVERSE_APPEND] >> simp[tbl2n_append_full] >> simp[Abbr`d0`] ) )
 
 val prefix_lem1 = Q.store_thm("prefix_lem1",
 `0<LENGTH b  ==> (a++b = c ==> a ≺c )`,
@@ -200,15 +200,15 @@ simp[prefix_def,rich_listTheory.IS_PREFIX_APPEND] >> rw[] >- (qexists_tac`b` >> 
 metis_tac[listTheory.NOT_NIL_EQ_LENGTH_NOT_0]  )
 
 val disjoint_pf_lem1 = Q.store_thm("disjoint_pf_lem1",
-`(TBL2N i * 2 ** (LENGTH j - LENGTH i) <= TBL2N j) ∧ (TBL2N j < (TBL2N i + 1) * 2 ** (LENGTH j - LENGTH i)) ∧ (LENGTH i < LENGTH j) ==> i ≺ j`,
-rw[TBL2N_exp2] >> qabbrev_tac`Δ=LENGTH j − LENGTH i` >> 
-`TBL2N (i ++ Fpow Δ) + (TBL2N j-TBL2N (i ++ Fpow Δ)) = TBL2N j` by simp[] >> 
-qabbrev_tac`δ=TBL2N j-TBL2N (i ++ Fpow Δ)` >> `δ<2**Δ` by (fs[RIGHT_ADD_DISTRIB] >> 
-  `TBL2N j - TBL2N i * 2 ** Δ < 2 ** Δ` by simp[] >> 
-  `TBL2N j − TBL2N (i ++ Fpow Δ) < 2**Δ` by simp[GSYM TBL2N_exp2] >> fs[Abbr`δ`] ) >> 
-`∃l. TBL2N l = δ ∧ LENGTH l = Δ ∧ TBL2N (i++Fpow Δ) +δ = TBL2N (i++l)` by simp[TBL2N_lem1] >> 
-`TBL2N (i ++ l) = TBL2N j` by simp[] >> `LENGTH (i++l) = LENGTH j` by simp[Abbr`Δ`] >> 
-`i++l = j` by metis_tac[TBL2N_inj_len] >> `0<LENGTH l` by simp[Abbr`Δ`] >> metis_tac[prefix_lem1] )
+`(TBL2N i * 2 ** (LENGTH j - LENGTH i) <= TBL2N j) /\ (TBL2N j < (TBL2N i + 1) * 2 ** (LENGTH j - LENGTH i)) /\ (LENGTH i < LENGTH j) ==> i ≺ j`,
+rw[TBL2N_exp2] >> qabbrev_tac`D=LENGTH j − LENGTH i` >> 
+`TBL2N (i ++ Fpow D) + (TBL2N j-TBL2N (i ++ Fpow D)) = TBL2N j` by simp[] >> 
+qabbrev_tac`d=TBL2N j-TBL2N (i ++ Fpow D)` >> `d<2**D` by (fs[RIGHT_ADD_DISTRIB] >> 
+  `TBL2N j - TBL2N i * 2 ** D < 2 ** D` by simp[] >> 
+  `TBL2N j − TBL2N (i ++ Fpow D) < 2**D` by simp[GSYM TBL2N_exp2] >> fs[Abbr`d`] ) >> 
+`?l. TBL2N l = d /\ LENGTH l = D /\ TBL2N (i++Fpow D) +d = TBL2N (i++l)` by simp[TBL2N_lem1] >> 
+`TBL2N (i ++ l) = TBL2N j` by simp[] >> `LENGTH (i++l) = LENGTH j` by simp[Abbr`D`] >> 
+`i++l = j` by metis_tac[TBL2N_inj_len] >> `0<LENGTH l` by simp[Abbr`D`] >> metis_tac[prefix_lem1] )
 
 val prefix_length_lt = Q.store_thm("prefix_length_lt",
 `a ≺ b ==> LENGTH a < LENGTH b`,
@@ -225,16 +225,16 @@ val TBL2N_append = Q.store_thm("TBL2N_append",
 simp[REVERSE_APPEND,tbl2n_append])
 
 val prefix_append= Q.store_thm("prefix_append",
-`a ≺ b <=> ∃s. b=a++s ∧ s<>[]`,
+`a ≺ b <=> ?s. b=a++s /\ s<>[]`,
 simp[prefix_def] >> rw[rich_listTheory.IS_PREFIX_APPEND,EQ_IMP_THM] >> metis_tac[APPEND_NIL,APPEND_EQ_SELF])
 
 val disjoint_prefix_free = Q.store_thm("disjoint_prefix_free",
-`prefix_free P <=> let is = IMAGE interval_bl P in ∀i1 i2. i1 ∈ is ∧ i2∈is ∧ i1<>i2 ==> disjoint_interval i1 i2`,
+`prefix_free P <=> let is = IMAGE interval_bl P in !i1 i2. i1 IN is /\ i2 IN is /\ i1<>i2 ==> disjoint_interval i1 i2`,
 rw[EQ_IMP_THM] 
 >- (rename[`interval_bl i = interval_bl j`] >> 
-    `¬(i ≺ j) ∧ ¬(j ≺ i)∧ i<>j` by metis_tac[prefix_free_def] >> 
+    `~(i ≺ j) /\ ~(j ≺ i)/\ i<>j` by metis_tac[prefix_free_def] >> 
     fs[interval_bl_def,disjoint_interval_def,DISJOINT_DEF,EXTENSION] >> 
-    rw[GSYM DISJ_ASSOC] >> rw[DECIDE``¬p∨q ⇔ p⇒q``] >> strip_tac >> 
+    rw[GSYM DISJ_ASSOC] >> rw[DECIDE``~p\/q <=> p==>q``] >> strip_tac >> 
     `LENGTH i <> LENGTH j` by (strip_tac >> fs[] >> qabbrev_tac`M = 2 rpow -&LENGTH j` >> 
       `&TBL2N i * M < &TBL2N j * M + M` by metis_tac[REAL_LET_TRANS] >>
       `&TBL2N j * M < &TBL2N i * M + M` by metis_tac[REAL_LET_TRANS] >>
@@ -260,7 +260,7 @@ rw[EQ_IMP_THM]
      (&TBL2N i +1)  * 2 rpow -&LENGTH i  * 2 rpow &LENGTH j` by 
        metis_tac[RPOW_POS_LT,REAL_LT_RMUL] >>
     fs[GSYM REAL_MUL_ASSOC,GSYM RPOW_ADD,RPOW_0,add_ints] >> rfs[] >>
-    qabbrev_tac`Δ=LENGTH j − LENGTH i` >> qabbrev_tac`ii= TBL2N i` >> 
+    qabbrev_tac`D=LENGTH j − LENGTH i` >> qabbrev_tac`ii= TBL2N i` >> 
     qabbrev_tac`jj= TBL2N j` >> fs[GSYM GEN_RPOW,REAL_OF_NUM_POW] >> 
     fs[disjoint_pf_lem1])
 >- (fs[prefix_free_def,PULL_EXISTS] >>rw[] >>
@@ -293,7 +293,7 @@ rw[interval_bl_def])
 
 val TBL2N_append_sing_ub = Q.store_thm("TBL2N_append_sing_ub",
 `&(TBL2N (a++[h]) + 1)*2 rpow (-1) <= &(TBL2N a + 1)`,
-`&(2 * TBL2N a + 2) * 2 rpow -1 ≤ &(TBL2N a + 1)` by  
+`&(2 * TBL2N a + 2) * 2 rpow -1 <= &(TBL2N a + 1)` by  
   (`&(2 * TBL2N a + 2) * 2 rpow -1 = &(2*(TBL2N a + 1)) * 2 rpow -1` by fs[GSYM LEFT_ADD_DISTRIB]>> 
    `_ = 2 * &(TBL2N a + 1) * 2 rpow -1` by fs[REAL_MUL] >> 
    `_ = &(TBL2N a + 1)*(2 rpow 1 * 2 rpow -1)`by 
@@ -306,7 +306,7 @@ Cases_on`h` >> rw[TBL2N_append] >>
 irule REAL_LE_TRANS >> qexists_tac`&(2 * TBL2N a + 2) * 2 rpow -1` >> rw[] )
 
 val interval_bl_bounds = Q.store_thm("interval_bl_bounds",
-`0<= FST (interval_bl a) ∧ FST (interval_bl a) + SND (interval_bl a) <= 1`,
+`0<= FST (interval_bl a) /\ FST (interval_bl a) + SND (interval_bl a) <= 1`,
 rw[] >- (fs[interval_bl_def] >> `(0:real)<= &TBL2N a` by fs[tbl2n_def] >> `(0:real)<2` by simp[] >>
          `0<2 rpow -&LENGTH a` by fs[RPOW_POS_LT] >> 
          metis_tac[util_probTheory.REAL_LE_LT_MUL] )
@@ -318,22 +318,22 @@ rw[] >- (fs[interval_bl_def] >> `(0:real)<= &TBL2N a` by fs[tbl2n_def] >> `(0:re
         simp[GSYM REAL_MUL_ASSOC,GSYM RPOW_ADD,RPOW_0,GSYM GEN_RPOW,REAL_OF_NUM_POW] >> 
         (TBL2N_ub |> Q.INST [`l`|->`a`] |> assume_tac) >> simp[]  ) )
 
-val bls_size_def = Define`bls_size (P:bool list -> bool) n = SIGMA (λs. (2 rpow -&LENGTH s)) {x|x ∈ P ∧ LENGTH x < n }`
+val bls_size_def = Define`bls_size (P:bool list -> bool) n = SIGMA (\s. (2 rpow -&LENGTH s)) {x|x IN P /\ LENGTH x < n }`
 
 val finite_bool_list_lt_n = Q.store_thm("finite_bool_list_lt_n",
 `FINITE {(s:bool list) | LENGTH s < n}`,
 Induct_on`n` >> simp[finite_bool_list_n] >> 
 `FINITE {(s:bool list)|LENGTH s = n}` by fs[finite_bool_list_n] >> 
-`FINITE ({(s:bool list) | LENGTH s < n ∨ LENGTH s = n}) ` by simp[FINITE_UNION,GSPEC_OR] >> 
-`{(s:bool list) | LENGTH s < SUC n} = {s | LENGTH s < n ∨ LENGTH s = n}` by rw[EXTENSION] >>fs[])
+`FINITE ({(s:bool list) | LENGTH s < n \/ LENGTH s = n}) ` by simp[FINITE_UNION,GSPEC_OR] >> 
+`{(s:bool list) | LENGTH s < SUC n} = {s | LENGTH s < n \/ LENGTH s = n}` by rw[EXTENSION] >>fs[])
 
 val finite_and = Q.store_thm("finite_and",
-`FINITE {s| P s} ==> FINITE {s|  Q s ∧ P s}`,
-rw[] >> `{s | Q s ∧ P s} = {s | Q s}  ∩ {s | P s}` by fs[INTER_DEF] >> fs[FINITE_INTER])
+`FINITE {s| P s} ==> FINITE {s|  Q s /\ P s}`,
+rw[] >> `{s | Q s /\ P s} = {s | Q s}  INTER {s | P s}` by fs[INTER_DEF] >> fs[FINITE_INTER])
 
 val interval_bl_sigma = Q.store_thm("interval_bl_sigma",
-`FINITE  {x | x ∈ P} ==> 
-SIGMA (λa. SND (interval_bl a)) {x | x ∈ P} = SIGMA (λa. 2 rpow -&LENGTH a) {x | x ∈ P} `,
+`FINITE  {x | x IN P} ==> 
+SIGMA (\a. SND (interval_bl a)) {x | x IN P} = SIGMA (\a. 2 rpow -&LENGTH a) {x | x IN P} `,
 rw[] >> irule REAL_SUM_IMAGE_EQ >> rw[] >> simp[interval_bl_def]);
 
 
@@ -343,12 +343,12 @@ fun fsr thl = full_simp_tac(srw_ss () ++ realSimps.REAL_ARITH_ss) thl;
 
 val disjoint_interval_thm = Q.store_thm("disjoint_interval_thm",
 `disjoint_interval (interval_bl i) (interval_bl j) ==> 
-FST (interval_bl i) + SND (interval_bl i) <= FST (interval_bl j) ∨ 
+FST (interval_bl i) + SND (interval_bl i) <= FST (interval_bl j) \/ 
 FST (interval_bl j) + SND (interval_bl j) <= FST (interval_bl i)`,
 rw[interval_bl_def,disjoint_interval_def,DISJOINT_DEF,EXTENSION,PULL_EXISTS] >> 
 Cases_on` &TBL2N i * 2 rpow -&LENGTH i + 2 rpow -&LENGTH i < &TBL2N j * 2 rpow -&LENGTH j` >> 
 fsr[]>> 
-qabbrev_tac`id=2 rpow -&LENGTH i` >> qmatch_abbrev_tac`_ ∨ jj+jd<=ii:real` >>
+qabbrev_tac`id=2 rpow -&LENGTH i` >> qmatch_abbrev_tac`_ \/ jj+jd<=ii:real` >>
 spose_not_then assume_tac >>
 fsr[REAL_NOT_LT,REAL_NOT_LE]  >> 
 first_x_assum(fn th => qspec_then`jj` assume_tac th >> qspec_then`ii` assume_tac th) >> fsr[]
@@ -358,11 +358,11 @@ first_x_assum(fn th => qspec_then`jj` assume_tac th >> qspec_then`ii` assume_tac
     `0<jd` suffices_by metis_tac[REAL_LET_TRANS,REAL_LT_REFL] >> simp[Abbr`jd`,RPOW_POS_LT]) )
 
 
-val max_rs_lemma = Q.prove(`∀s. FINITE s ==> s<>{} ==> ∃x:real. x∈s ∧ ∀y. y∈s ==> y<=x`,
+val max_rs_lemma = Q.prove(`!s. FINITE s ==> s<>{} ==> ?x:real. x IN s /\ !y. y IN s ==> y<=x`,
 Induct_on`FINITE` >>rw[] >> Cases_on`s={}` >> fs[] >> qexists_tac`max e x` >> fsr[max_def] >> rw[]
 >- metis_tac[] >> Cases_on`y=e`>> fsr[] >> RES_TAC >> fsr[] )
 
-val min_rs_lemma = Q.prove(`∀s. FINITE s ==> s<>{} ==> ∃x:real. x∈s ∧ ∀y. y∈s ==> x<=y`,
+val min_rs_lemma = Q.prove(`!s. FINITE s ==> s<>{} ==> ?x:real. x IN s /\ !y. y IN s ==> x<=y`,
 Induct_on`FINITE` >>rw[] >> Cases_on`s={}` >> fs[] >> qexists_tac`min e x` >> fsr[min_def] >> rw[]>>
 Cases_on`y=e`>> fsr[] >> RES_TAC >> fsr[] )
 
@@ -372,10 +372,10 @@ SIMP_RULE(srw_ss() )[SKOLEM_THM,GSYM RIGHT_EXISTS_IMP_THM] max_rs_lemma)
 val minr_set_def = new_specification("minr_set_def",["minr_set"],
 SIMP_RULE(srw_ss() )[SKOLEM_THM,GSYM RIGHT_EXISTS_IMP_THM] min_rs_lemma)
 
-val exten_def = Define`exten s = (minr_set {FST k| k ∈ s},maxr_set {FST k + SND k|k∈s})`
+val exten_def = Define`exten s = (minr_set {FST k| k IN s},maxr_set {FST k + SND k|k IN s})`
 
 val maxr_set_thm = Q.store_thm("maxr_set_thm[simp]",
-`maxr_set {e} = e ∧ (FINITE s ∧ s<> {} ==> maxr_set (e INSERT s) = max e (maxr_set s))`,
+`maxr_set {e} = e /\ (FINITE s /\ s<> {} ==> maxr_set (e INSERT s) = max e (maxr_set s))`,
 rw[] >- (qspec_then `{e}` mp_tac maxr_set_def >> simp[]) >> 
 qspec_then `e INSERT s` mp_tac maxr_set_def  >> simp[] >> strip_tac >> 
 qabbrev_tac`m = maxr_set (e INSERT s)` >> qspec_then`s` mp_tac maxr_set_def >> simp[] >> 
@@ -385,19 +385,19 @@ qabbrev_tac`m0 = maxr_set s` >> rw[] >> rw[max_def]
 spose_not_then strip_assume_tac >> `m<=m0` by fsr[] >> `m<e` by fsr[] >> `e<=m` by fsr[] >> fsr[])
 
 val minr_set_thm = Q.store_thm("minr_set_thm[simp]",
-`minr_set {e} = e ∧ (FINITE s ∧ s<> {} ==> minr_set (e INSERT s) = min e (minr_set s))`,
+`minr_set {e} = e /\ (FINITE s /\ s<> {} ==> minr_set (e INSERT s) = min e (minr_set s))`,
 rw[] >- (qspec_then `{e}` mp_tac minr_set_def >> simp[]) >> 
 qspec_then `e INSERT s` mp_tac minr_set_def  >> simp[] >> strip_tac >> 
 qabbrev_tac`m = minr_set (e INSERT s)` >> qspec_then`s` mp_tac minr_set_def >> simp[] >> 
 qabbrev_tac`m0 = minr_set s` >> rw[] >> rw[min_def] 
 >- (Cases_on`e = m0` >> rw[] >- (simp[Abbr`m`,ABSORPTION_RWT]) >> Cases_on`e=m` >> rw[] >>
-    `m<=e` by metis_tac[] >>`m∈s` by fs[] >>`m0<=m` by fs[] >> metis_tac[REAL_LE_ANTISYM]) >> 
+    `m<=e` by metis_tac[] >>`m IN s` by fs[] >>`m0<=m` by fs[] >> metis_tac[REAL_LE_ANTISYM]) >> 
 spose_not_then strip_assume_tac >> `m<=m0` by fsr[] >> `m0<e` by fsr[] >> `m<=e` by fsr[] >> 
 Cases_on`m=e` >> fsr[] >> `m0 <= m` by fsr[] >> fsr[])
 
 val maxr_set_union = Q.store_thm("maxr_set_union",
-`∀s1. (FINITE s1) ==> ∀s2. (FINITE s2) ==> (s1 <> ∅ ∧  s2 <> ∅) ==> 
-  maxr_set (s1 ∪ s2)=max (maxr_set s1) (maxr_set s2)`,
+`!s1. (FINITE s1) ==> !s2. (FINITE s2) ==> (s1 <> EMPTY /\  s2 <> EMPTY ) ==> 
+  maxr_set (s1 UNION s2)=max (maxr_set s1) (maxr_set s2)`,
 Induct_on`FINITE` >> strip_tac
 >- (Induct_on`FINITE` >>rw[maxr_set_thm] )
 >- (ntac 4 strip_tac >> Induct_on`FINITE` >> rw[maxr_set_thm] >> 
@@ -415,8 +415,8 @@ Induct_on`FINITE` >> strip_tac
 
 
 val minr_set_union = Q.store_thm("minr_set_union",
-`∀s1. (FINITE s1) ==> ∀s2. (FINITE s2) ==> (s1 <> ∅ ∧  s2 <> ∅) ==> 
-  minr_set (s1 ∪ s2)=min (minr_set s1) (minr_set s2)`,
+`!s1. (FINITE s1) ==> !s2. (FINITE s2) ==> (s1 <> EMPTY /\  s2 <> EMPTY ) ==> 
+  minr_set (s1 UNION s2)=min (minr_set s1) (minr_set s2)`,
 Induct_on`FINITE` >> strip_tac
 >- (Induct_on`FINITE` >>rw[minr_set_thm] )
 >- (ntac 4 strip_tac >> Induct_on`FINITE` >> rw[minr_set_thm] >> 
@@ -428,40 +428,40 @@ Induct_on`FINITE` >> strip_tac
     >- (Cases_on`e<= minr_set s1` >> fs[min_def,minr_set_thm,INSERT_UNION_EQ] >> rw[] >> 
         fsr[] >> Cases_on`minr_set s1 <= e'` >> fsr[])
     >- (Cases_on`e<= minr_set s1` >> fs[min_def,minr_set_thm,INSERT_UNION_EQ] >> rw[] >> 
-        fsr[] >> Cases_on` minr_set s1 ≤ e'` >>rw[] >> fsr[])
+        fsr[] >> Cases_on` minr_set s1 <= e'` >>rw[] >> fsr[])
     >- (fs[min_def,minr_set_thm,INSERT_UNION_EQ]) )
 )
 
 
 val gspec_eq = Q.store_thm("gspec_eq[simp]",
-`GSPEC (λx. (f x,x=k)) = {f k}`,
+`GSPEC (\x. (f x,x=k)) = {f k}`,
 simp[EXTENSION])
 
 val gspec_in = Q.store_thm("gspec_in[simp]",
-`GSPEC (λx. (f x,x∈k)) = {f x|x∈k}`,
+`GSPEC (\x. (f x,x IN k)) = {f x|x IN k}`,
 simp[EXTENSION])
 
 val gspec_f_or = Q.store_thm("gspec_f_or[simp]",
-`∀P Q. {f x | P x ∨ Q x} = {f x | P x} ∪ {f x | Q x}`,
+`!P Q. {f x | P x \/ Q x} = {f x | P x} UNION {f x | Q x}`,
 rw[IN_UNION,EXTENSION] >> metis_tac[GSPECIFICATION_applied])
 
 
 
 val exten_insert_thm = Q.store_thm("exten_insert_thm",
-`(s <> ∅ ∧ FINITE s) ==> exten (e INSERT s) =  (min (FST e) ## max (FST e + SND e)) (exten s)`,
+`(s <> EMPTY /\ FINITE s) ==> exten (e INSERT s) =  (min (FST e) ## max (FST e + SND e)) (exten s)`,
 simp[exten_def,maxr_set_thm,minr_set_thm] >> rw[] 
->- (`{FST k | k <> e ==> k ∈ s} = {FST k | k = e ∨ k ∈ s}` by fs[EXTENSION] >>
-    `{FST k | k = e ∨ k ∈ s} = {FST k | k = e} ∪ {FST k | k ∈ s}` by fs[] >> rw[] >> 
+>- (`{FST k | k <> e ==> k IN s} = {FST k | k = e \/ k IN s}` by fs[EXTENSION] >>
+    `{FST k | k = e \/ k IN s} = {FST k | k = e} UNION {FST k | k IN s}` by fs[] >> rw[] >> 
     `FINITE {FST e}` by fs[] >> `{FST e} <> {}` by fs[] >> 
-    `FINITE {FST k | k ∈ s}` by metis_tac[IMAGE_FINITE,IMAGE_DEF] >> 
-    `{FST k | k ∈ s} <> {}` by metis_tac[IMAGE_EQ_EMPTY,IMAGE_DEF]>>
+    `FINITE {FST k | k IN s}` by metis_tac[IMAGE_FINITE,IMAGE_DEF] >> 
+    `{FST k | k IN s} <> {}` by metis_tac[IMAGE_EQ_EMPTY,IMAGE_DEF]>>
     rw[minr_set_union])
->- (`{FST k + SND k | k <> e ==> k ∈ s} = {FST k + SND k | k = e ∨ k ∈ s}` by fs[EXTENSION] >>
-    `{FST k + SND k | k = e ∨ k ∈ s} = {FST k + SND k | k = e} ∪ {FST k + SND k | k ∈ s}` by fs[] >> 
+>- (`{FST k + SND k | k <> e ==> k IN s} = {FST k + SND k | k = e \/ k IN s}` by fs[EXTENSION] >>
+    `{FST k + SND k | k = e \/ k IN s} = {FST k + SND k | k = e} UNION {FST k + SND k | k IN s}` by fs[] >> 
     rw[] >> 
     `FINITE {FST e  + SND k}` by fs[] >> `{FST e  + SND k} <> {}` by fs[] >> 
-    `FINITE {FST k + SND k | k ∈ s}` by metis_tac[IMAGE_FINITE,IMAGE_DEF] >> 
-    `{FST k + SND k | k ∈ s} <> {}` by metis_tac[IMAGE_EQ_EMPTY,IMAGE_DEF]>>
+    `FINITE {FST k + SND k | k IN s}` by metis_tac[IMAGE_FINITE,IMAGE_DEF] >> 
+    `{FST k + SND k | k IN s} <> {}` by metis_tac[IMAGE_EQ_EMPTY,IMAGE_DEF]>>
     rw[maxr_set_union] ))
 
 val TBL2N_ub2 = Q.store_thm("TBL2N_ub2",
@@ -482,9 +482,9 @@ drule_then (ONCE_REWRITE_TAC o list_of_singleton o GSYM) REAL_LE_RMUL >>
 simp[REAL_ADD_RDISTRIB,GSYM REAL_MUL_ASSOC,GSYM RPOW_ADD,RPOW_0,GSYM GEN_RPOW,REAL_OF_NUM_POW])
 
 val lemma11 = Q.store_thm("lemma11",
-`∀s. FINITE s ==> (∀x dx y dy. (x,dx)∈s ∧ (y,dy) ∈ s ∧ x<>y ==> x+dx<=y ∨ y+dy<=x) ∧
-              (∀x d. (x,d)∈s ==> 0r<d) ∧ (∀x d. (x,d)∈s ==> 0<= x ∧ x+d <=1) ∧ (s <> {}) 
-          ==> (0<= FST (exten s) ∧ SND (exten s) <= 1)`,
+`!s. FINITE s ==> (!x dx y dy. (x,dx) IN s /\ (y,dy) IN s /\ x<>y ==> x+dx<=y \/ y+dy<=x) /\
+              (!x d. (x,d) IN s ==> 0r<d) /\ (!x d. (x,d) IN s ==> 0<= x /\ x+d <=1) /\ (s <> {}) 
+          ==> (0<= FST (exten s) /\ SND (exten s) <= 1)`,
 Induct_on`FINITE` >> simp[] >>ntac 2 (gen_tac>>strip_tac) >>strip_tac >> Cases_on`s={}` >> fs[]
 >- (simp[maxr_set_def,minr_set_def,exten_def,ITSET_THM] >> Cases_on`e` >> fs[]) >>
 fs[exten_insert_thm] >> rw[max_def,min_def]
@@ -506,7 +506,7 @@ val interval_bl_inj = Q.store_thm("interval_bl_inj",
 `INJ interval_bl P (IMAGE interval_bl P)`,
 simp[INJ_DEF])
 
-val lemma12 = Q.prove(`bls_size P n = SIGMA SND (IMAGE interval_bl {s|s ∈ P ∧ LENGTH s < n})`,
+val lemma12 = Q.prove(`bls_size P n = SIGMA SND (IMAGE interval_bl {s|s IN P /\ LENGTH s < n})`,
 fs[bls_size_def,interval_bl_def,REAL_SUM_IMAGE_IMAGE,interval_bl_inj,finite_bool_list_lt_n,finite_and,combinTheory.o_DEF])
 
 val exten_sing = Q.store_thm("exten_sing[simp]",
@@ -514,17 +514,17 @@ val exten_sing = Q.store_thm("exten_sing[simp]",
 fs[exten_def])
 
 val size_of_exten = Q.prove(
-`∀s. FINITE s ==> (∀x dx y dy. (x,dx)∈s ∧ (y,dy) ∈ s ∧ (x,dx)<>(y,dy) ==> x+dx<=y ∨ y+dy<=x) ∧
-              (∀x d. (x,d)∈s ==> 0r<d) ∧ (s <> {}) 
+`!s. FINITE s ==> (!x dx y dy. (x,dx) IN s /\ (y,dy) IN s /\ (x,dx)<>(y,dy) ==> x+dx<=y \/ y+dy<=x) /\
+              (!x d. (x,d) IN s ==> 0r<d) /\ (s <> {}) 
           ==> SIGMA SND s <= SND (exten s) - FST (exten s)`,
 HO_MATCH_MP_TAC FINITE_COMPLETE_INDUCTION >> rw[] >> 
-map_every qabbrev_tac[`Rs = {FST k + SND k | k∈s}`,`Ls = {FST k |k∈s}`]>>
+map_every qabbrev_tac[`Rs = {FST k + SND k | k IN s}`,`Ls = {FST k |k IN s}`]>>
 `FINITE Ls` by metis_tac[IMAGE_FINITE,IMAGE_DEF] >>
 `Ls <> {}` by metis_tac[IMAGE_EQ_EMPTY,IMAGE_DEF] >>
-`∃e1 e2. (e1,e2)∈s ∧ ∀m. m∈ Ls ==> e1<=m` 
-  by (qexists_tac `minr_set Ls` >> qexists_tac`@e'. (minr_set Ls,e')∈s` >> reverse(rw[])
+`?e1 e2. (e1,e2) IN s /\ !m. m IN Ls ==> e1<=m` 
+  by (qexists_tac `minr_set Ls` >> qexists_tac`@e'. (minr_set Ls,e') IN s` >> reverse(rw[])
       >- (metis_tac[minr_set_def]) >> SELECT_ELIM_TAC >> simp[] >> 
-      `minr_set Ls ∈ Ls` by metis_tac[minr_set_def] >> fs[Abbr`Ls`] >> 
+      `minr_set Ls IN Ls` by metis_tac[minr_set_def] >> fs[Abbr`Ls`] >> 
       metis_tac[pairTheory.PAIR]) >>
 qabbrev_tac`s0 = s DELETE (e1,e2)` >> Cases_on`s0={}` >> simp[] 
   >- (`s = {(e1,e2)}` by (metis_tac[DELETE_EQ_SING]) >> rw[REAL_SUM_IMAGE_THM] >> fsr[]) >> 
@@ -534,50 +534,50 @@ qabbrev_tac`s0 = s DELETE (e1,e2)` >> Cases_on`s0={}` >> simp[]
 fsr[REAL_SUM_IMAGE_THM] >> 
 `SND (exten s0) - FST (exten s0) <=  SND (exten ((e1,e2) INSERT s0)) − FST (exten ((e1,e2) INSERT s0)) - e2` suffices_by fsr[] >> 
 fsr[exten_def,exten_insert_thm,REAL_SUM_IMAGE_THM,DELETE_NON_ELEMENT_RWT] >>
-map_every qabbrev_tac [`MX = maxr_set {FST k + SND k | k ∈ s0}`,`MN = minr_set  {FST k | k ∈ s0}`]>>
-map_every qabbrev_tac[`Rs0 = {FST k + SND k | k∈s0}`,`Ls0 = {FST k |k∈s0}`] >>
+map_every qabbrev_tac [`MX = maxr_set {FST k + SND k | k IN s0}`,`MN = minr_set  {FST k | k IN s0}`]>>
+map_every qabbrev_tac[`Rs0 = {FST k + SND k | k IN s0}`,`Ls0 = {FST k |k IN s0}`] >>
 `FINITE Ls0` by metis_tac[IMAGE_FINITE,IMAGE_DEF] >>
 `Ls0 <> {}` by metis_tac[IMAGE_EQ_EMPTY,IMAGE_DEF] >>
-`MN ∈ Ls0` by metis_tac[minr_set_def] >>
-`∃n. (MN,n)∈s0` by (`∃p. p∈s0 ∧ FST p = MN` suffices_by (rw[] >> metis_tac[pairTheory.PAIR]) >>
+`MN IN Ls0` by metis_tac[minr_set_def] >>
+`?n. (MN,n) IN s0` by (`?p. p IN s0 /\ FST p = MN` suffices_by (rw[] >> metis_tac[pairTheory.PAIR]) >>
                     pop_assum MP_TAC >> simp[Abbr`Ls0`] >> metis_tac[]) >>
-`MN ∈ Ls` by (simp[Abbr`Ls`] >>metis_tac[pairTheory.FST]) >>
+`MN IN Ls` by (simp[Abbr`Ls`] >>metis_tac[pairTheory.FST]) >>
 rw[max_def,min_def] >> fsr[]
 >- (`e1 + e2 <= MN` suffices_by fsr[] >> 
     first_x_assum(qspecl_then[`e1`,`e2`,`MN`,`n`] MP_TAC) >> simp[] >> impl_tac
     >- (rpt strip_tac >> rw[] >> rw[Abbr`s0`] >> fs[]) >> strip_tac >> `e1<=MN` by fs[]>>
      `0<n` suffices_by fsr[] >> metis_tac[]  )
 >- (`MX < e1+e2` by fsr[] >> `FINITE Rs0` by metis_tac[IMAGE_FINITE,IMAGE_DEF] >>
-    `Rs0 <> {}` by metis_tac[IMAGE_EQ_EMPTY,IMAGE_DEF] >>`MX ∈ Rs0` by metis_tac[maxr_set_def]>>
-    `∃i j. (i,j)∈s0 ∧ MX = i+j` by (pop_assum MP_TAC >> simp[Abbr`Rs0`] >> 
+    `Rs0 <> {}` by metis_tac[IMAGE_EQ_EMPTY,IMAGE_DEF] >>`MX IN Rs0` by metis_tac[maxr_set_def]>>
+    `?i j. (i,j) IN s0 /\ MX = i+j` by (pop_assum MP_TAC >> simp[Abbr`Rs0`] >> 
                                     metis_tac[pairTheory.PAIR]) >> 
     first_x_assum(qspecl_then[`e1`,`e2`,`i`,`j`] MP_TAC) >> simp[] >> impl_tac
     >- (rpt strip_tac >> rw[] >> rw[Abbr`s0`] >> fs[]) >> strip_tac
     >- (rw[] >> `0<j` suffices_by fsr[] >> metis_tac[]) >> rw[] >> 
-    `i∈Ls` by (simp[Abbr`Ls`,pairTheory.EXISTS_PROD] >>metis_tac[])>> `e1<=i` by simp[]>>
+    `i IN Ls` by (simp[Abbr`Ls`,pairTheory.EXISTS_PROD] >>metis_tac[])>> `e1<=i` by simp[]>>
     `0<j` suffices_by fsr[] >> metis_tac[]  ) )
 
 
 val exten_member = Q.store_thm("exten_member",
-`FINITE s ∧ s <> {} ∧ exten (s) = (sn,sx) ==> 
- (∃sn' sx' dx. (sn,sn') ∈ s ∧ (sx',dx)∈ s ∧ sx'+dx=sx)`,
-simp[exten_def] >> rw[] >> `{FST k|k∈s} = IMAGE FST s` by simp[EXTENSION] >> 
-`FINITE {FST k|k ∈ s} ∧ {FST k | k∈s} <> {}` by simp[] >> drule_all minr_set_def >>rw[] >> 
+`FINITE s /\ s <> {} /\ exten (s) = (sn,sx) ==> 
+ (?sn' sx' dx. (sn,sn') IN s /\ (sx',dx) IN s /\ sx'+dx=sx)`,
+simp[exten_def] >> rw[] >> `{FST k|k IN s} = IMAGE FST s` by simp[EXTENSION] >> 
+`FINITE {FST k|k IN s} /\ {FST k | k IN s} <> {}` by simp[] >> drule_all minr_set_def >>rw[] >> 
 qexists_tac`SND k` >> simp[] >> 
-`{FST k + SND k|k∈s} = IMAGE (λk. FST k+ SND k) s` by simp[EXTENSION] >> 
-`FINITE {FST k + SND k|k ∈ s} ∧ {FST k + SND k | k∈s} <> {}` by simp[] >> drule_all maxr_set_def >>
+`{FST k + SND k|k IN s} = IMAGE (\k. FST k+ SND k) s` by simp[EXTENSION] >> 
+`FINITE {FST k + SND k|k IN s} /\ {FST k + SND k | k IN s} <> {}` by simp[] >> drule_all maxr_set_def >>
 rw[] >> rename[`maxr_set _ = FST kk + SND kk`] >> map_every qexists_tac [`FST kk`,`SND kk`] >> simp[])
 
-val _ = overload_on ("bpos" ,`` λl. &TBL2N l * 2 rpow -&LENGTH l``);
+val _ = overload_on ("bpos" ,`` \l. &TBL2N l * 2 rpow -&LENGTH l``);
 
 val bpos_min = Q.store_thm("bpos_min",
-`∀s. FINITE s ==> s <> {} ==> ∃l. l∈s ∧ ∀m. m∈s ==> bpos l <= bpos m`,
+`!s. FINITE s ==> s <> {} ==> ?l. l IN s /\ !m. m IN s ==> bpos l <= bpos m`,
 Induct_on`FINITE` >> simp[] >> rw[] >> Cases_on`s={}` >> simp[] >>fs[] >> Cases_on`bpos e <= bpos l`>>
 fs[] >- (qexists_tac`e` >> simp[] >> metis_tac[REAL_LE_TRANS,REAL_LE_REFL]) >> qexists_tac`l` >>
 simp[] >> metis_tac[REAL_NOT_LE,REAL_LT_IMP_LE] )
 
 val exten_low_high = Q.store_thm("exten_low_high",
-`∀s. FINITE s ==> s <> {} ==> ∀low high. exten (IMAGE interval_bl s) = (low,high) ==> low <= high`,
+`!s. FINITE s ==> s <> {} ==> !low high. exten (IMAGE interval_bl s) = (low,high) ==> low <= high`,
 Induct_on`FINITE` >> simp[] >> rw[] >> Cases_on`s={}` >> simp[] >>fs[]
 >- (fs[interval_bl_def] >> rw[REAL_LE_ADDR] >> rw[RPOW_POS_LT,REAL_LE_LT]) >>
 qpat_x_assum`exten _ = _` mp_tac >> rfs[exten_insert_thm] >> Cases_on`exten (IMAGE interval_bl s)` >>
@@ -585,13 +585,13 @@ fs[] >> fsr[interval_bl_def,min_def,max_def] >> rw[]>>fsr[] )
 
 
 
-val lemma13 = Q.store_thm("lemma13",`∀P. FINITE P ==> (P <> {}) ==>
-                           (∀x y. x ∈ P ∧ y ∈ P ∧ x ≠ y ⇒ 
+val lemma13 = Q.store_thm("lemma13",`!P. FINITE P ==> (P <> {}) ==>
+                           (!x y. x IN P /\ y IN P /\ x <> y ==> 
                                   disjoint_interval (interval_bl x) (interval_bl y)) ==> 
-                           (SIGMA (λs. 2 rpow -&LENGTH s) P + FST (exten (IMAGE interval_bl P) ) 
+                           (SIGMA (\s. 2 rpow -&LENGTH s) P + FST (exten (IMAGE interval_bl P) ) 
                             <= SND (exten (IMAGE interval_bl P) ))`,
 HO_MATCH_MP_TAC FINITE_COMPLETE_INDUCTION >> rw[] >>qmatch_abbrev_tac`_ <= SND (exten s)` >>
-`∃l. l ∈ P ∧ ∀m. m∈P ==> bpos l <= bpos m` by metis_tac[bpos_min] >> 
+`?l. l IN P /\ !m. m IN P ==> bpos l <= bpos m` by metis_tac[bpos_min] >> 
 qabbrev_tac`P0 = P DELETE l` >> Cases_on`P0={}` >> simp[] 
   >- (`P = {l}` by (metis_tac[DELETE_EQ_SING]) >> 
       fsr[REAL_SUM_IMAGE_THM,Abbr`s`,interval_bl_def,REAL_LE_ADDL,TBL2N_lb]) >>
@@ -599,11 +599,11 @@ qabbrev_tac`P0 = P DELETE l` >> Cases_on`P0={}` >> simp[]
 >- (rw[Abbr`P0`] >> metis_tac[]) >>`P = l INSERT P0` by fs[Abbr`P0`] >> 
 `P0 DELETE l = P0` by fs[Abbr`P0`,ELT_IN_DELETE,DELETE_NON_ELEMENT] >>
 fsr[REAL_SUM_IMAGE_THM,Abbr`s`,exten_insert_thm] >>
-`∃en ex. exten (IMAGE interval_bl P0) = (en,ex)` by metis_tac[pairTheory.pair_CASES] >> simp[]>>
-`∃l0 d. interval_bl l = (l0,d)` by metis_tac[pairTheory.pair_CASES] >> fs[] >> 
+`?en ex. exten (IMAGE interval_bl P0) = (en,ex)` by metis_tac[pairTheory.pair_CASES] >> simp[]>>
+`?l0 d. interval_bl l = (l0,d)` by metis_tac[pairTheory.pair_CASES] >> fs[] >> 
 `2 rpow -&LENGTH l = d` by fsr[interval_bl_def] >> fs[] >>
 `max (l0 + d) ex = d + max l0 (ex-d)` by (fsr[max_def] >> rw[] >> fsr[]) >>fsr[GSYM REAL_ADD_ASSOC]>>
-`∃en'. (en,en')∈ IMAGE interval_bl P0` by metis_tac[exten_member,IMAGE_FINITE,IMAGE_EQ_EMPTY]>> fs[]>>
+`?en'. (en,en') IN IMAGE interval_bl P0` by metis_tac[exten_member,IMAGE_FINITE,IMAGE_EQ_EMPTY]>> fs[]>>
 rename[`(en,en') = interval_bl EN`] >>
 `l0+d<=en` by (first_x_assum (qspecl_then [`l`,`EN`] mp_tac) >> 
              simp[] >> impl_tac >- (strip_tac >> fs[GSYM DELETE_NON_ELEMENT])  >> 
@@ -618,60 +618,62 @@ rename[`(en,en') = interval_bl EN`] >>
 fsr[max_def] )
 
 val lemma1 = Q.prove(
-`(let is = IMAGE interval_bl P in ∀i1 i2. i1 ∈ is ∧ i2∈is ∧ i1<>i2 ==> disjoint_interval i1 i2)
- ==>(∀n. bls_size P n <= 1)`,
+`(let is = IMAGE interval_bl P in !i1 i2. i1 IN is /\ i2 IN is /\ i1<>i2 ==> disjoint_interval i1 i2)
+ ==>(!n. bls_size P n <= 1)`,
 rw[EQ_IMP_THM,PULL_EXISTS] >> fs[bls_size_def,disjoint_interval_thm] >> 
-`FINITE  {x | x ∈ P ∧ LENGTH x < n}` by metis_tac[finite_and,finite_bool_list_lt_n] >>
-`FINITE {(λy. (&TBL2N y * 2 rpow -&LENGTH y,2 rpow -&LENGTH y)) x| x∈ {z | z ∈ P ∧ LENGTH z <n}}`
+`FINITE  {x | x IN P /\ LENGTH x < n}` by metis_tac[finite_and,finite_bool_list_lt_n] >>
+`FINITE {(\y. (&TBL2N y * 2 rpow -&LENGTH y,2 rpow -&LENGTH y)) x| x IN {z | z IN P /\ LENGTH z <n}}`
  by metis_tac[IMAGE_FINITE,IMAGE_DEF] >> fs[] >> 
-qabbrev_tac`s = {(&TBL2N x * 2 rpow -&LENGTH x,2 rpow -&LENGTH x) |  x ∈ P ∧ LENGTH x < n}` >>
+qabbrev_tac`s = {(&TBL2N x * 2 rpow -&LENGTH x,2 rpow -&LENGTH x) |  x IN P /\ LENGTH x < n}` >>
 Cases_on`s={}` 
->- (`{x | x ∈ P ∧ LENGTH x < n} = {}` by (fs[Abbr`s`] >> 
-      `{(λy. (&TBL2N y * 2 rpow -&LENGTH y,2 rpow -&LENGTH y))  x | x ∈ P ∧ LENGTH x < n} = {}`
+>- (`{x | x IN P /\ LENGTH x < n} = {}` by (fs[Abbr`s`] >> 
+      `{(\y. (&TBL2N y * 2 rpow -&LENGTH y,2 rpow -&LENGTH y))  x | x IN P /\ LENGTH x < n} = {}`
         by simp[] >> 
-      `IMAGE (λx. (&TBL2N x * 2 rpow -&LENGTH x,2 rpow -&LENGTH x)) {x | x ∈ P ∧ LENGTH x < n}
-        = {(λy. (&TBL2N y * 2 rpow -&LENGTH y,2 rpow -&LENGTH y))  x | x ∈ P ∧ LENGTH x < n}`
+      `IMAGE (\x. (&TBL2N x * 2 rpow -&LENGTH x,2 rpow -&LENGTH x)) {x | x IN P /\ LENGTH x < n}
+        = {(\y. (&TBL2N y * 2 rpow -&LENGTH y,2 rpow -&LENGTH y))  x | x IN P /\ LENGTH x < n}`
         by fs[IMAGE_DEF] >> metis_tac[IMAGE_EQ_EMPTY]) >> fs[REAL_SUM_IMAGE_THM] ) >> 
-`0<= FST (exten s) ∧ SND (exten s) <= 1` by 
+`0<= FST (exten s) /\ SND (exten s) <= 1` by 
   (irule lemma11 >> rw[]>> fsr[Abbr`s`,TBL2N_lb,rpow_len_lb,TBL2N_ub2] >> 
    rw[] >> `x'<>x''` by (metis_tac[FUN_EQ_THM]) >> 
    `disjoint_interval (interval_bl x') (interval_bl x'')` by simp[] >> 
-   `FST (interval_bl x') + SND (interval_bl x') ≤ FST (interval_bl x'') ∨
-     FST (interval_bl x'') + SND (interval_bl x'') ≤ FST (interval_bl x')` by 
+   `FST (interval_bl x') + SND (interval_bl x') <= FST (interval_bl x'') \/
+     FST (interval_bl x'') + SND (interval_bl x'') <= FST (interval_bl x')` by 
      simp[disjoint_interval_thm]  >> fs[interval_bl_def] ) >> 
 qmatch_abbrev_tac`SIGMA f sn <= 1r`>> `SIGMA f sn <= SND (exten s)` suffices_by fsr[] >> 
 `s = IMAGE interval_bl sn` by (fs[Abbr`sn`,Abbr`s`,interval_bl_def,IMAGE_DEF]) >> rw[] >>
-`∀x x'. x ∈ sn ∧ x' ∈ sn ∧ x ≠ x' ⇒
+`!x x'. x IN sn /\ x' IN sn /\ x <> x' ==>
              disjoint_interval (interval_bl x) (interval_bl x')` by 
-  (`sn = P ∩ {x | LENGTH x < n}` by fs[INTER_DEF] >> rw[]) >> 
+  (`sn = P INTER {x | LENGTH x < n}` by fs[INTER_DEF] >> rw[]) >> 
 Cases_on`sn={}` >> fs[REAL_SUM_IMAGE_THM] >>
 `SIGMA f sn + FST (exten (IMAGE interval_bl sn)) <= SND (exten (IMAGE interval_bl sn))` by 
   fs[Abbr`f`,lemma13] >> fsr[] )
 
 val kraft_ineq1 = Q.store_thm("kraft_ineq1",
-`∀P. prefix_free P ==> (∀n. bls_size P n <= 1)`,
-(* Could change to `∃y0. y0<=1 ∧ bls_size P --> y0` *)
+`!P. prefix_free P ==> (!n. bls_size P n <= 1)`,
+(* Could change to `?y0. y0<=1 /\ bls_size P --> y0` *)
  metis_tac[disjoint_prefix_free,lemma1])
  
-(*  In progress of proving *)
 
-(*
+(*  TO DO AT SOME POINT
 
-val numl_size_def = Define`numl_size L n = SIGMA (λs. (2 rpow -&s)) {x|x ∈ L ∧ x < n }`
+val numl_size_def = Define`numl_size L = FOLDR (\n A. A+(2 rpow -&n)) 0 L`
+
+val kraft_conv_cw_def = Define`kraft_conv_cw C i =  `
 
 val kraft_ineq_conv = Q.store_thm("kraft_ineq_conv",
-`∀L. (∃y0. y0<=1 ∧ numl_size L --> y0) ==> 
-(∃P. prefix_free P ∧ (∀p. p∈P ==> ∃l. l∈L ∧ LENGTH p = l) ∧ (∀l. l∈L ==> ∃p. p∈P ∧ LENGTH p=l ) )`,
-) 
+`!L. numl_size L <= 1 ==> 
+(?P b. prefix_free P /\ BIJ b (count (LENGTH L) ) P  /\  !i. i < LENGTH L ==> LENGTH (b i) = EL i L)`,
+rw[] >> `?CLIST. CLIST = SET_TO_LIST L` by fs[SET_TO_LIST_THM] >> qexists_tac`` ) 
 
+*)
 
 (* Have done initial Kolmog stuff *)
 
 val prefix_machine_def = Define`prefix_machine (U:bool list -> extnat) = 
-                                ∃P. prefix_free P∧(∀x. x ∈ P <=> ∃y. U x = SOME y)`
+                                ?P. prefix_free P/\(!x. x IN P <=> ?y. U x = SOME y)`
 
 val monotone_machine_def = Define`monotone_machine (U:bool list -> extnat) = 
-                     ∀p1 p2. ∃x1 x2. (U p1 = (SOME x1)) ∧ (U p2 = (SOME x2)) ==> (p1 ≼ p2 ==> (n2bl x1 ≼ n2bl x2 ∨ n2bl x2 ≼ n2bl x1) )`
+                     !p1 p2 x1 x2. (U p1 = (SOME x1)) /\ (U p2 = (SOME x2)) ==> (p1 ≼ p2 ==> (n2bl x1 ≼ n2bl x2 \/ n2bl x2 ≼ n2bl x1) )`
 
 val kolmog_complexity_def = Define`kolmog_complexity x U =
                        if  { p | U p = SOME x} = {} then NONE
@@ -680,11 +682,10 @@ val kolmog_complexity_def = Define`kolmog_complexity x U =
 val prefix_kolmog_complexity_def = Define`pkolmog_complexity x U = 
                                 if prefix_machine U then kolmog_complexity x U else NONE`
 
-(* Mono def not working right now  *)
 val monotone_kolmog_complexity_def = Define`mkolmog_complexity x U = 
                                 if monotone_machine U then 
-                                  if ∀y. { p | (U p = SOME y) ∧ (x ≼ (n2bl y)) } = {} then NONE
-                                   else SOME (MIN_SET {LENGTH p |∃y. (U p = SOME y) ∧(x ≼ n2bl y)}) 
+                                  if  { p | ?y. (U p = SOME y) /\ (x ≼ (n2bl y)) } = {} then NONE
+                                   else SOME (MIN_SET {LENGTH p | ?y. (U p = SOME y) /\(x ≼ n2bl y)}) 
                                 else NONE`
 
 val kolmog_def = Define`kolmog x = kolmog_complexity x universal_tm`
@@ -705,23 +706,142 @@ val cond_kolmog_complexity_def = Define`cond_kolmog_complexity x y U =
 val cond_kolmog_def = Define`cond_kolmog x y = cond_kolmog_complexity x y universal_tm`
 
 
+val tpow_append = Q.store_thm("tpow_append",
+`Tpow (a+b) = Tpow a ++ Tpow b`,
+ONCE_REWRITE_TAC[ADD_COMM] >> fs[Tpow_def,GENLIST_APPEND,combinTheory.K_DEF])
+
+val tpow_suc = Q.store_thm("tpow_suc",
+`Tpow (SUC a) = T::(Tpow a)`,
+fs[Tpow_def,GENLIST_CONS])
+
+val prefix_free_bar = Q.store_thm("prefix_free_bar",
+`prefix_free (IMAGE bar s)`,
+fs[prefix_free_def,PULL_EXISTS] >> rw[] >> rename[`bar x ≺ bar y`] >> simp[bar_def] >> strip_tac >>
+fs[prefix_append] >> 
+`LENGTH x = LENGTH y` by 
+  (`¬(LENGTH x < LENGTH y) ∧¬(LENGTH y < LENGTH x)` suffices_by simp[] >> rpt strip_tac
+   >-(`∃i. LENGTH y = LENGTH x + i ∧ 0<i` by intLib.ARITH_TAC >> 
+      full_simp_tac bool_ss[GSYM APPEND_ASSOC,APPEND_11,tpow_append] >> Cases_on`i` >> fs[tpow_suc])
+   >-(`∃i. LENGTH x = LENGTH y + i ∧ 0<i` by intLib.ARITH_TAC >> 
+      full_simp_tac bool_ss[GSYM APPEND_ASSOC,APPEND_11,tpow_append] >> Cases_on`i` >> fs[tpow_suc]))>>full_simp_tac bool_ss[GSYM APPEND_ASSOC,APPEND_11] >> 
+first_x_assum(mp_tac o AP_TERM``LENGTH:bool list -> num``) >> simp[] >> Cases_on`s'` >> fs[]  )
+
+val unbar_def = Define`unbar [] = [] ∧
+                       unbar (T::x) = unbar x ∧
+                       unbar (F::x) = x `;
+
+
+val unbar_tpow = Q.store_thm("unbar_tpow",
+`unbar (Tpow n ++ x) = unbar x`,
+simp[Tpow_def] >> Induct_on`n` >> simp[unbar_def,GENLIST_CONS])
+
+val unbar_bar_inv = Q.store_thm("bar_unbar_inv[simp]",
+`∀x. unbar (bar x) = x `,
+fs[bar_def] >> REWRITE_TAC[GSYM APPEND_ASSOC,unbar_tpow,APPEND,unbar_def])
+
+val barred_def = Define`barred x = ∃y. x=bar y`
+
+val bar2_def = Define`bar2 (x,y) = (bar x) ++ (bar y)`
+
+val bar2ed_def = Define`bar2ed x = ∃y z. x = (bar y)++z`
+
+val unbar2_def = Define`unbar2 i (T::rest) = unbar2 (i+1) rest ∧
+                        unbar2 i (F::rest) = (TAKE i rest,DROP i rest)`
+
+val unbar2_induct_bar2 = Q.store_thm("unbar2_induct_bar2",
+`∀i. unbar2 i (Tpow j ++ F::rest) = (TAKE (i+j) rest,DROP (i+j) rest)`,
+simp[Tpow_def] >> Induct_on`j` >> simp[unbar2_def,GENLIST_CONS,ADD1]) 
+
 (** up to here **)
 (* In Process of proving   *)
 
+val unbar2_bar2_inv = Q.store_thm("unbar2_bar_inv",
+`unbar2 0 (bar2 x) = x`,
+Cases_on`x` >> rw[bar2_def,bar_def] >> REWRITE_TAC [GSYM APPEND_ASSOC,APPEND,unbar2_induct_bar2]>>
+simp[] >>
+`LENGTH q <= LENGTH q` by fs[] >> 
+`TAKE (LENGTH q) (q ++  (Tpow (LENGTH r) ++ [F] ++ r)) = q ++ TAKE (LENGTH q − LENGTH q)  (Tpow (LENGTH r) ++ [F] ++ r)` by metis_tac[rich_listTheory.TAKE_APPEND2] >>
+`DROP (LENGTH q) (q ++ (Tpow (LENGTH r) ++ [F] ++ r)) = DROP (LENGTH q − LENGTH q) (Tpow (LENGTH r) ++ [F] ++ r)` by metis_tac[rich_listTheory.DROP_APPEND2] >> fs[Once (GSYM APPEND_ASSOC)] >>
+metis_tac[GSYM APPEND_ASSOC]
+)
 
+
+
+val prefix_rec_fun_def = Define`prefix_rec_fun i = prefix_free (IMAGE n2bl {x|Phi i x <> NONE})`
+
+val nbar_def = Define`nbar n = bl2n (bar (n2bl n))`
+
+val pr_log2_def = Define`pr_log2 = WFM (λf n. if n<=1 then 1 else 1+(f (n DIV 2)) )`
+
+val pr_log2_pr = Q.store_thm("pr_log2_pr",
+`primrec (pr_log2) 1`,
+simp[pr_log2_def] >> irule primrec_WFM >> irule primrec_pr2 >> simp[restr_def]>>
+qexists_tac`` )
+
+val pr_nbar = Q.store_thm("pr_nbar",
+`nbar n = n* 2**(pr_log2 [n] +1)+ (3*2**(pr_log2 [n])) - 1 `,
+Induct_on`n` >> simp[nbar_def])
+
+val recfn_nbar = Q.store_thm("recfn_nbar",
+`recfn (rec1 (SOME o nbar)) 1`,
+irule recfn_rec1 >> qexists_tac`SOME o (λl. nbar (HD l))` >> rw[] >> irule primrec_recfn >>
+)
+
+(* f will be nbar *)
+(* U will num_unbar then call recPhi on the undone npair *)
+
+val num_unbar_def = Define`num_unbar n = bl2n (unbar (n2bl n))`
+
+val pfU_def = Define`pfU = rec1 (λn. let m = num_unbar n in recPhi [nfst m;nsnd m])`
+
+val prefix_rec_fun_exists = Q.store_thm("prefix_rec_fun_exists",
+`∃U. prefix_rec_fun U`,
+qexists_tac`UMi` >> simp[prefix_rec_fun_def] >> simp[UMi_def,nlist_of_onto])
+
+val prefix_universal_rec_fun = Q.store_thm("prefix_universal_rec_fun",
+`∃U f. ∀x y. Phi f (npair x y) <> NONE ∧ Phi U (THE (Phi f (npair x y))) = Phi x y  ∧ prefix_rec_fun U`
+)
+
+
+
+
+val pref_utm_def = Define`pref_utm p = if bar2ed p then 
+                                         (let (a,b) = unbar2 0 p in Phi (bl2n a) (bl2n b)) 
+				       else NONE`
+
+val prefix_pref_utm = Q.store_thm("prefix_pref_utm",
+`prefix_machine pref_utm`,
+simp[prefix_machine_def] >> qexists_tac` IMAGE bar {x| universal_tm x <> NONE}` >> 
+rw[prefix_free_bar] >> rw[pref_utm_def]>>
+eq_tac  >>rw[]
+>- (simp[barred_def] >> metis_tac[optionTheory.option_CASES])
+>- (fs[barred_def] >> rw[] >> fs[] >>  metis_tac[optionTheory.NOT_SOME_NONE])  )
+
+
+val pref_utm_is_universal = Q.store_thm("pref_utm_is_universal",
+`pr_is_universal (pref_utm o n2bl)`,
+fs[pr_is_universal_def,pref_utm_def] >> rw[]
+>- ()
+>- (simp[bldemunge_inv] >> qexists_tac `SOME o proj 0` >> 
+    simp[recfn_rules,bldmunge_bld_eq,bool_list_to_num_def] >> rw[] >>
+    Induct_on`y` >> simp[blpair_encode_def,blmunge_def,unbar2_def,Once num_to_bool_list_def,Once bool_list_to_num_def]  )
+
+
+assume_tac(SIMP_RULE (srw_ss())[LET_THM] universal_Phi ) >> 
+fs[universal_tm_def,combinTheory.o_DEF,pref_utm_def])
 
 (*
 
-val leastR_def = Define`leastR R A = @a. a IN A ∧ ∀b. b IN A ==> ~R b a`
+val leastR_def = Define`leastR R A = @a. a IN A /\ !b. b IN A ==> ~R b a`
 
-val order_def = tDefine"order"`(order A R 0 = leastR R A) ∧
-                (order A R (SUC n) = leastR R (A DIFF IMAGE (λi. order A R i) (count (SUC n))))`(WF_REL_TAC`measure (SND o SND)` >> simp[])
+val order_def = tDefine"order"`(order A R 0 = leastR R A) /\
+                (order A R (SUC n) = leastR R (A DIFF IMAGE (\i. order A R i) (count (SUC n))))`(WF_REL_TAC`measure (SND o SND)` >> simp[])
 
 val tmorder_def = Define`tmorder x = order {p | universal_tm p = x} `
 
-val listlex_def = Define`(listlex [] x <=> x<>[])∧(listlex (h::t) [] <=> F)∧
+val listlex_def = Define`(listlex [] x <=> x<>[])/\(listlex (h::t) [] <=> F)/\
                          (listlex (h1::t1) (h2::t2) <=>
-			 (LENGTH t1 < LENGTH t2) ∨ ((LENGTH t1 = LENGTH t2) ∧ ((h1=h2) ∧ listlex t1 t2 ∨ ~h1 ∧ h2 )  ) )`
+			 (LENGTH t1 < LENGTH t2) \/ ((LENGTH t1 = LENGTH t2) /\ ((h1=h2) /\ listlex t1 t2 \/ ~h1 /\ h2 )  ) )`
 
 val listlex_length = Q.store_thm("listlex_length",
 `!a b. LENGTH a < LENGTH b ==> listlex a b`,
@@ -737,11 +857,11 @@ val listlex_empty = Q.store_thm("listlex_empty[simp]",
 Cases_on `a` >> simp[listlex_def])
 
 val listlex_same_length = Q.store_thm("listlex_same_length",
-`!B l w. (!b. B b ==> (LENGTH b = l)) ∧ B w ==> ?v. B v ∧ (!b. listlex b v ==> ~B b)`,
+`!B l w. (!b. B b ==> (LENGTH b = l)) /\ B w ==> ?v. B v /\ (!b. listlex b v ==> ~B b)`,
 Induct_on `l` >> simp[] >- (rw[] >> qexists_tac`[]` >> simp[] >> metis_tac[]) >>
-rw[] >> Cases_on`?hf. B' hf ∧ (HD hf = F)`
+rw[] >> Cases_on`?hf. B' hf /\ (HD hf = F)`
 >- (fs[] >>
-    `?c. B' c ∧ (HD c= F) ∧ (!d. listlex d c ==> ~B' d)`
+    `?c. B' c /\ (HD c= F) /\ (!d. listlex d c ==> ~B' d)`
       by (first_x_assum(qspec_then`{t|B' (F::t)}`MP_TAC) >> simp[] >>
           disch_then(qspec_then`TL hf`MP_TAC) >> Cases_on `hf` >> simp[]
           >- (res_tac >> fs[]) >> fs[] >> impl_tac
@@ -760,10 +880,10 @@ rw[] >> Cases_on`?hf. B' hf ∧ (HD hf = F)`
 
 val WF_listlex = Q.store_thm("WF_listlex",`WF listlex`,
 simp[relationTheory.WF_DEF] >> rw[] >>
-`?v. B' v ∧ !v'. B' v' ==> LENGTH v <= LENGTH v'`
+`?v. B' v /\ !v'. B' v' ==> LENGTH v <= LENGTH v'`
   by (`WF (inv_image $< (LENGTH:bool list -> num) )` by (simp[relationTheory.WF_inv_image])>>
   fs[relationTheory.WF_DEF] >> metis_tac[NOT_LESS])>>
-  qspecl_then[`{l|B' l ∧ (LENGTH l = LENGTH v)}`,`LENGTH v`,`v`] MP_TAC listlex_same_length >>
+  qspecl_then[`{l|B' l /\ (LENGTH l = LENGTH v)}`,`LENGTH v`,`v`] MP_TAC listlex_same_length >>
   rw[] >> qexists_tac`v'` >> rw[] >> strip_tac >> `LENGTH b <> LENGTH v` by metis_tac[] >>
   `LENGTH v' < LENGTH b` by metis_tac[LESS_OR_EQ] >>
   `listlex v' b` by metis_tac[listlex_length] >>
@@ -778,14 +898,14 @@ val num_to_bool_list_def = tDefine"num_to_bool_list"`num_to_bool_list n =
 (WF_REL_TAC `$<` >> intLib.ARITH_TAC)
 
 val solomonoff_prior_def = Define`
-solomonoff_prior x = suminf (λn. let b = num_to_bool_list n in
+solomonoff_prior x = suminf (\n. let b = num_to_bool_list n in
 				     if universal_tm b = x
 				     then inv(2 pow (LENGTH b))
 				     else 0) `
 
 
 val existence_of_universal_semimeasure = Q.store_thm("existence_of_universal_semimeasure",
-`∃M. (semimeasure M) ∧ (universal_semimeasure M setX) ∧ (continous M) ∧ (lower_semicompute M)`,
+`?M. (semimeasure M) /\ (universal_semimeasure M setX) /\ (continous M) /\ (lower_semicompute M)`,
 qexists_tac `solomonoff_prior` >> conj_tac)
 
 val summed_square_error_a_def = Define`summed_square_a_error mu a n =
@@ -803,7 +923,7 @@ val KL_greater_hellinger = Q.store_thm("KL_greater_hellinger",
 `hellinger_dis P Q <= KL_dis P Q`,
 )
 
-val KL_M_dis_def = Define`KL_M_dis mu x = KL_dis (λy. cond_M y x) (λy. cond_mu y x)`
+val KL_M_dis_def = Define`KL_M_dis mu x = KL_dis (\y. cond_M y x) (\y. cond_mu y x)`
 
 val sum_KL_M_dis_def = Define`sum_KL_M_dis mu n = sum for (x:length x = n-1)
                                                   (mu x) * (KL_M_dis mu x)`
@@ -828,6 +948,6 @@ rw[LESS_EQ_TRANS,solomonoff_thm_claim_11,solomonoff_thm_claim_2])
  *)
 
 
-*)
+
 
 val _ = export_theory();
